specs/Spec.Exponentiation.fsti
@@ -11,37 +11,37 @@ module Loops = Lib.LoopCombinators
 #set-options "--z3rlimit 50 --fuel 0 --ifuel 0"
 
 inline_for_extraction
-class to_cm (t:Type) = {
+class to_comm_monoid (t:Type) = {
   a_spec: Type;
-  cm: S.comm_monoid a_spec;
+  comm_monoid: S.comm_monoid a_spec;
   refl: x:t -> a_spec;
 }
 
 
 inline_for_extraction
-let one_st (t:Type) (to:to_cm t) = unit -> Pure t
+let one_st (t:Type) (to:to_comm_monoid t) = unit -> Pure t
   (requires True)
   (ensures  fun one ->
-    to.refl one == to.cm.S.one)
+    to.refl one == to.comm_monoid.S.one)
 
 
 inline_for_extraction
-let mul_st (t:Type) (to:to_cm t) = x:t -> y:t -> Pure t
+let mul_st (t:Type) (to:to_comm_monoid t) = x:t -> y:t -> Pure t
   (requires True)
   (ensures  fun xy ->
-    to.refl xy == to.cm.S.mul (to.refl x) (to.refl y))
+    to.refl xy == to.comm_monoid.S.mul (to.refl x) (to.refl y))
 
 
 inline_for_extraction
-let sqr_st (t:Type) (to:to_cm t) = x:t -> Pure t
+let sqr_st (t:Type) (to:to_comm_monoid t) = x:t -> Pure t
   (requires True)
   (ensures  fun xy ->
-    to.refl xy == to.cm.S.mul (to.refl x) (to.refl x))
+    to.refl xy == to.comm_monoid.S.mul (to.refl x) (to.refl x))
 
 
 inline_for_extraction
 class concrete_ops (t:Type) = {
-  to: to_cm t;
+  to: to_comm_monoid t;
   one: one_st t to;
   mul: mul_st t to;
   sqr: sqr_st t to;
@@ -64,7 +64,7 @@ let exp_rl (#t:Type) (k:concrete_ops t) (a:t) (bBits:nat) (b:nat{b < pow2 bBits}
 
 
 val exp_rl_lemma: #t:Type -> k:concrete_ops t -> a:t -> bBits:nat -> b:nat{b < pow2 bBits} ->
-  Lemma (k.to.refl (exp_rl k a bBits b) == S.exp_rl k.to.cm (k.to.refl a) bBits b)
+  Lemma (k.to.refl (exp_rl k a bBits b) == S.exp_rl k.to.comm_monoid (k.to.refl a) bBits b)
 
 
 let exp_mont_ladder_swap_f (#t:Type) (k:concrete_ops t)
@@ -85,7 +85,7 @@ let exp_mont_ladder_swap (#t:Type) (k:concrete_ops t) (a:t) (bBits:nat) (b:nat{b
 
 
 val exp_mont_ladder_swap_lemma: #t:Type -> k:concrete_ops t -> a:t -> bBits:nat -> b:nat{b < pow2 bBits} ->
-  Lemma (k.to.refl (exp_mont_ladder_swap k a bBits b) == S.exp_mont_ladder_swap k.to.cm (k.to.refl a) bBits b)
+  Lemma (k.to.refl (exp_mont_ladder_swap k a bBits b) == S.exp_mont_ladder_swap k.to.comm_monoid (k.to.refl a) bBits b)
 
 
 let exp_pow2 (#t:Type) (k:concrete_ops t) (a:t) (b:nat) : t =
@@ -93,7 +93,7 @@ let exp_pow2 (#t:Type) (k:concrete_ops t) (a:t) (b:nat) : t =
 
 
 val exp_pow2_lemma: #t:Type -> k:concrete_ops t -> a:t -> b:nat ->
-  Lemma (k.to.refl (exp_pow2 k a b) == S.exp_pow2 k.to.cm (k.to.refl a) b)
+  Lemma (k.to.refl (exp_pow2 k a b) == S.exp_pow2 k.to.comm_monoid (k.to.refl a) b)
 
 
 let rec pow (#t:Type) (k:concrete_ops t) (a:t) (b:nat) : t =
@@ -108,7 +108,7 @@ val pow_unfold: #t:Type -> k:concrete_ops t -> a:t -> i:pos ->
   Lemma (pow k a i == k.mul a (pow k a (i - 1)))
 
 val pow_lemma: #t:Type -> k:concrete_ops t -> a:t -> b:nat ->
-  Lemma (k.to.refl (pow k a b) == S.pow k.to.cm (k.to.refl a) b)
+  Lemma (k.to.refl (pow k a b) == S.pow k.to.comm_monoid (k.to.refl a) b)
 
 
 let exp_fw_acc0 (#t:Type0) (k:concrete_ops t) (a:t)
@@ -139,7 +139,7 @@ let exp_fw (#t:Type) (k:concrete_ops t) (a:t) (bBits:nat) (b:nat{b < pow2 bBits}
 
 
 val exp_fw_lemma: #t:Type -> k:concrete_ops t -> a:t -> bBits:nat -> b:nat{b < pow2 bBits} -> l:pos ->
-  Lemma (k.to.refl (exp_fw k a bBits b l) == S.exp_fw k.to.cm (k.to.refl a) bBits b l)
+  Lemma (k.to.refl (exp_fw k a bBits b l) == S.exp_fw k.to.comm_monoid (k.to.refl a) bBits b l)
 
 
 let exp_double_fw_acc0 (#t:Type) (k:concrete_ops t)
@@ -176,4 +176,4 @@ val exp_double_fw_lemma: #t:Type -> k:concrete_ops t
   -> a1:t -> bBits:nat -> b1:nat{b1 < pow2 bBits}
   -> a2:t -> b2:nat{b2 < pow2 bBits} -> l:pos ->
   Lemma (k.to.refl (exp_double_fw k a1 bBits b1 a2 b2 l) ==
-    S.exp_double_fw k.to.cm (k.to.refl a1) bBits b1 (k.to.refl a2) b2 l)
+    S.exp_double_fw k.to.comm_monoid (k.to.refl a1) bBits b1 (k.to.refl a2) b2 l)
